more porting

Weidenbach_Book/CDCL_WNOT.thy
@@ -1,5 +1,5 @@
 theory CDCL_WNOT
-imports CDCL_NOT CDCL_W_Termination
+imports CDCL_NOT CDCL_W_Termination CDCL_W_Merge
 begin
 
 section \<open>Link between Weidenbach's and NOT's CDCL\<close>
@@ -101,17 +101,12 @@ sublocale state\<^sub>W \<subseteq> dpll_state
    "\<lambda>C S. remove_cls C S"
    by unfold_locales (auto simp: map_tl o_def)
 
+
+
 context state\<^sub>W
 begin
 declare state_simp\<^sub>N\<^sub>O\<^sub>T[simp del]
 
-definition inv\<^sub>N\<^sub>O\<^sub>T :: "'st \<Rightarrow> bool" where
-"inv\<^sub>N\<^sub>O\<^sub>T \<equiv> \<lambda>S. no_dup (trail S)"
-
-declare inv\<^sub>N\<^sub>O\<^sub>T_def[simp]
-
-definition backjump_l_cond :: "'v clause \<Rightarrow> 'v clause \<Rightarrow> 'v literal \<Rightarrow> 'st \<Rightarrow> 'st \<Rightarrow> bool"  where
-"backjump_l_cond = (\<lambda> _ _ _ _ _. True)"
 end
 
 sublocale conflict_driven_clause_learning\<^sub>W \<subseteq> cdcl\<^sub>N\<^sub>O\<^sub>T_merge_bj_learn_ops
@@ -128,12 +123,6 @@ sublocale conflict_driven_clause_learning\<^sub>W \<subseteq> cdcl\<^sub>N\<^sub
   "\<lambda>C C' L' S T. backjump_l_cond C C' L' S T
     \<and> distinct_mset (C' + {#L'#}) \<and> \<not>tautology (C' + {#L'#})"
   by unfold_locales
-
-context conflict_driven_clause_learning\<^sub>W
-begin
-declare [[show_abbrevs = false]]
-term backjump_l
-end
 
 thm cdcl\<^sub>N\<^sub>O\<^sub>T_merge_bj_learn_proxy.axioms
 sublocale conflict_driven_clause_learning\<^sub>W \<subseteq> cdcl\<^sub>N\<^sub>O\<^sub>T_merge_bj_learn_proxy
@@ -189,20 +178,17 @@ next
           true_clss_cls_remdups_mset union_commute)
       have "F \<Turnstile>as CNot (remdups_mset C')"
         by (simp add: \<open>F \<Turnstile>as CNot C'\<close>)
-      show ?thesis sorry
-(*       have "Ex (backjump_l S)"
+      obtain D where D: "mset_cls D = remdups_mset C' + {#L#}"
+        using ex_mset_cls by blast
+      have "Ex (backjump_l S)"
         apply standard
-        apply (rule backjump_l.intros[OF  _ f2])
+        apply (rule backjump_l.intros[OF  _ f2, of _ _ _ ])
         using f4 f3 f2 \<open>\<not> tautology (remdups_mset C' + {#L#})\<close>
         calculation(2-5,9) \<open>F \<Turnstile>as CNot (remdups_mset C')\<close>
-        state_eq\<^sub>N\<^sub>O\<^sub>T_ref unfolding backjump_l_cond_def by auto
+        state_eq\<^sub>N\<^sub>O\<^sub>T_ref D unfolding backjump_l_cond_def by blast+
       then show ?thesis
-        using f4 f3 f2 \<open>\<not> tautology (remdups_mset C' + {#L#})\<close>
-        backjump_l.intros[OF  _ f2] calculation(2-5,9)
-        state_eq\<^sub>N\<^sub>O\<^sub>T_ref unfolding backjump_l_cond_def by blast
-      qed
- *)
-  qed
+        by blast
+    qed
 qed
 
 sublocale conflict_driven_clause_learning\<^sub>W \<subseteq> cdcl\<^sub>N\<^sub>O\<^sub>T_merge_bj_learn_proxy2  _ _ _ _ _ _ _ _ _
@@ -258,6 +244,50 @@ lemma reduce_trail_to\<^sub>N\<^sub>O\<^sub>T_reduce_trail_convert:
   apply (induction C S rule: reduce_trail_to\<^sub>N\<^sub>O\<^sub>T.induct)
   apply (subst reduce_trail_to\<^sub>N\<^sub>O\<^sub>T.simps, subst reduce_trail_to.simps)
   by auto
+
+lemma reduce_trail_to_map[simp]: 
+  "reduce_trail_to (map f M) S = reduce_trail_to M S"
+  by (rule reduce_trail_to_length) simp
+
+(* TODO Move to CDCL_NOT *)
+lemma reduce_trail_to\<^sub>N\<^sub>O\<^sub>T_length:
+  "length M = length M' \<Longrightarrow> reduce_trail_to\<^sub>N\<^sub>O\<^sub>T M S = reduce_trail_to\<^sub>N\<^sub>O\<^sub>T M' S"
+  apply (induction M S arbitrary:  rule: reduce_trail_to\<^sub>N\<^sub>O\<^sub>T.induct)
+  by (simp add: reduce_trail_to\<^sub>N\<^sub>O\<^sub>T.simps)
+
+lemma reduce_trail_to\<^sub>N\<^sub>O\<^sub>T_map[simp]: 
+  "reduce_trail_to\<^sub>N\<^sub>O\<^sub>T (map f M) S = reduce_trail_to\<^sub>N\<^sub>O\<^sub>T M S"
+  by (rule reduce_trail_to\<^sub>N\<^sub>O\<^sub>T_length) simp
+
+lemma skip_or_resolve_state_change:
+  assumes "skip_or_resolve\<^sup>*\<^sup>* S T"
+  shows
+    "\<exists>M. trail S = M @ trail T \<and> (\<forall>m \<in> set M. \<not>is_marked m)"
+    "clauses S = clauses T"
+    "backtrack_lvl S = backtrack_lvl T"
+  using assms 
+proof (induction rule: rtranclp_induct)
+  case base
+  case 1 show ?case by simp
+  case 2 show ?case by simp
+  case 3 show ?case by simp
+next
+  case (step T U) note st = this(1) and s_o_r = this(2) and IH = this(3) and IH' = this(3-5)
+  
+  case 2 show ?case using IH' s_o_r by (auto elim!: rulesE simp: skip_or_resolve.simps)
+  case 3 show ?case using IH' s_o_r by (auto elim!: rulesE simp: skip_or_resolve.simps)  
+  case 1 show ?case 
+    using s_o_r
+    proof cases
+      case s_or_r_skip
+      then show ?thesis using IH by (auto elim!: rulesE simp: skip_or_resolve.simps)  
+    next
+      case s_or_r_resolve
+      then show ?thesis 
+        using IH by (cases "trail T") (auto elim!: rulesE simp: skip_or_resolve.simps dest!:
+        hd_raw_trail)
+    qed
+qed
 
 subsection \<open>More lemmas conflict--propagate and backjumping\<close>
 subsection \<open>CDCL FW\<close>
@@ -399,9 +429,7 @@ next
         raw_clauses_def
         by (simp add: atms_of_def image_subset_iff)
       obtain M where tr_T: "trail T = M @ trail T'"
-        using s_or_r
-        by (induction rule: rtranclp_induct) (auto simp: skip_or_resolve.simps
-          elim!: rulesE)
+        using s_or_r skip_or_resolve_state_change by meson
       obtain M' where
         tr_T': "trail T' = M' @  Marked K (i+1) # tl (trail U)" and
         tr_U: "trail U = Propagated L (mset_ccls D) # tl (trail U)"
@@ -422,9 +450,9 @@ next
           apply (auto dest!: get_all_marked_decomposition_exists_prepend
             elim!: conflictE)
           by (rule sym) auto
-      ultimately have [simp]: "trail (reduce_trail_to\<^sub>N\<^sub>O\<^sub>T (convert_trail_from_W M1) S) = M1"
-        using M1_M2 confl
-        by (auto simp add: reduce_trail_to\<^sub>N\<^sub>O\<^sub>T_reduce_trail_convert comp_def)
+      ultimately have [simp]: "trail (reduce_trail_to\<^sub>N\<^sub>O\<^sub>T M1 S) = M1"
+        using M1_M2 confl by (subst reduce_trail_to\<^sub>N\<^sub>O\<^sub>T_reduce_trail_convert)
+        (auto simp: comp_def elim: rulesE)
       have "every_mark_is_a_conflict U"
         using inv_U unfolding cdcl\<^sub>W_all_struct_inv_def cdcl\<^sub>W_conflicting_def by simp
       then have U_D: "tl (trail U) \<Turnstile>as CNot (remove1_mset L (mset_ccls D))"
@@ -435,7 +463,7 @@ next
                  using tr_T apply simp
                 using inv unfolding cdcl\<^sub>W_all_struct_inv_def cdcl\<^sub>W_M_level_inv_def
                 apply (simp add: comp_def)
-               using U M1_M2 confl undef_L M1_M2 inv_T' inv unfolding cdcl\<^sub>W_all_struct_inv_def
+               using U M1_M2 confl undef_L M1_M2 inv_T' inv undef_L unfolding cdcl\<^sub>W_all_struct_inv_def
                cdcl\<^sub>W_M_level_inv_def apply (auto simp: state_eq\<^sub>N\<^sub>O\<^sub>T_def
                  trail_reduce_trail_to\<^sub>N\<^sub>O\<^sub>T_add_learned_cls)[]
               using C\<^sub>S apply auto[]
@@ -520,8 +548,8 @@ proof -
     proof cases
       case merged
       then show ?thesis
-        using cdcl\<^sub>N\<^sub>O\<^sub>T_decreasing_measure'[OF _ _ atm_clauses] atm_trail n_d
-        by (auto split: if_split simp: comp_def)
+        using cdcl\<^sub>N\<^sub>O\<^sub>T_decreasing_measure'[OF _ _ atm_clauses, of T] atm_trail n_d
+        by (auto split: if_split simp: comp_def image_image)
     next
       case n_s
       then show ?thesis by simp
@@ -532,6 +560,122 @@ lemma wf_cdcl\<^sub>W_merge: "wf {(T, S). cdcl\<^sub>W_all_struct_inv S \<and> c
   apply (rule wfP_if_measure[of _ _ "\<mu>\<^sub>F\<^sub>W"])
   using cdcl\<^sub>W_merge_\<mu>\<^sub>F\<^sub>W_decreasing by blast
 
+sublocale conflict_driven_clause_learning\<^sub>W_termination
+  by unfold_locales (simp add: wf_cdcl\<^sub>W_merge)
+
+lemma full_cdcl\<^sub>W_s'_full_cdcl\<^sub>W_merge_restart:
+  assumes
+    "conflicting R = None" and
+    inv: "cdcl\<^sub>W_all_struct_inv R"
+  shows "full cdcl\<^sub>W_s' R V \<longleftrightarrow> full cdcl\<^sub>W_merge_stgy R V" (is "?s' \<longleftrightarrow> ?fw")
+proof
+  assume ?s'
+  then have "cdcl\<^sub>W_s'\<^sup>*\<^sup>* R V" unfolding full_def by blast
+  have "cdcl\<^sub>W_all_struct_inv V"
+    using \<open>cdcl\<^sub>W_s'\<^sup>*\<^sup>* R V\<close> inv rtranclp_cdcl\<^sub>W_all_struct_inv_inv rtranclp_cdcl\<^sub>W_s'_rtranclp_cdcl\<^sub>W
+    by blast
+  then have n_s: "no_step cdcl\<^sub>W_merge_stgy V"
+    using no_step_cdcl\<^sub>W_s'_no_step_cdcl\<^sub>W_merge_stgy by (meson \<open>full cdcl\<^sub>W_s' R V\<close> full_def)
+  have n_s_bj: "no_step cdcl\<^sub>W_bj V"
+    by (metis \<open>cdcl\<^sub>W_all_struct_inv V\<close> \<open>full cdcl\<^sub>W_s' R V\<close> bj full_def
+      n_step_cdcl\<^sub>W_stgy_iff_no_step_cdcl\<^sub>W_cl_cdcl\<^sub>W_o)
+  have n_s_cp: "no_step cdcl\<^sub>W_merge_cp V"
+    proof -
+      { fix ss :: 'st
+        obtain ssa :: "'st \<Rightarrow> 'st" where
+          ff1: "\<forall>s. \<not> cdcl\<^sub>W_all_struct_inv s \<or> cdcl\<^sub>W_s'_without_decide s (ssa s)
+            \<or> no_step cdcl\<^sub>W_merge_cp s"
+          using conflicting_true_no_step_s'_without_decide_no_step_cdcl\<^sub>W_merge_cp by moura
+        have "(\<forall>p s sa. \<not> full p (s::'st) sa \<or> p\<^sup>*\<^sup>* s sa \<and> no_step p sa)" and
+          "(\<forall>p s sa. (\<not> p\<^sup>*\<^sup>* (s::'st) sa \<or> (\<exists>s. p sa s)) \<or> full p s sa)"
+          by (meson full_def)+
+        then have "\<not> cdcl\<^sub>W_merge_cp V ss"
+          using ff1 by (metis (no_types) \<open>cdcl\<^sub>W_all_struct_inv V\<close> \<open>full cdcl\<^sub>W_s' R V\<close> cdcl\<^sub>W_s'.simps
+            cdcl\<^sub>W_s'_without_decide.cases) }
+      then show ?thesis
+        by blast
+    qed
+  consider
+      (fw_no_confl) "cdcl\<^sub>W_merge_stgy\<^sup>*\<^sup>* R V" and "conflicting V = None"
+    | (fw_confl) "cdcl\<^sub>W_merge_stgy\<^sup>*\<^sup>* R V" and "conflicting V \<noteq> None" and "no_step cdcl\<^sub>W_bj V"
+    | (fw_dec_confl) S T U where "cdcl\<^sub>W_merge_stgy\<^sup>*\<^sup>* R S" and "no_step cdcl\<^sub>W_merge_cp S" and
+        "decide S T" and "cdcl\<^sub>W_merge_cp\<^sup>*\<^sup>* T U" and "conflict U V"
+    | (fw_dec_no_confl) S T where "cdcl\<^sub>W_merge_stgy\<^sup>*\<^sup>* R S" and "no_step cdcl\<^sub>W_merge_cp S" and
+        "decide S T" and "cdcl\<^sub>W_merge_cp\<^sup>*\<^sup>* T V" and "conflicting V = None"
+    | (cp_no_confl) "cdcl\<^sub>W_merge_cp\<^sup>*\<^sup>* R V" and "conflicting V = None"
+    | (cp_confl) U where "cdcl\<^sub>W_merge_cp\<^sup>*\<^sup>* R U" and "conflict U V"
+    using rtranclp_cdcl\<^sub>W_s'_no_step_cdcl\<^sub>W_s'_without_decide_decomp_into_cdcl\<^sub>W_merge[OF
+      \<open>cdcl\<^sub>W_s'\<^sup>*\<^sup>* R V\<close> assms] by auto
+  then show ?fw
+    proof cases
+      case fw_no_confl
+      then show ?thesis using n_s unfolding full_def by blast
+    next
+      case fw_confl
+      then show ?thesis using n_s unfolding full_def by blast
+    next
+      case fw_dec_confl
+      have "cdcl\<^sub>W_merge_cp U V"
+        using n_s_bj by (metis cdcl\<^sub>W_merge_cp.simps full_unfold fw_dec_confl(5))
+      then have "full1 cdcl\<^sub>W_merge_cp T V"
+        unfolding full1_def by (metis fw_dec_confl(4) n_s_cp tranclp_unfold_end)
+      then have "cdcl\<^sub>W_merge_stgy S V" using \<open>decide S T\<close> \<open>no_step cdcl\<^sub>W_merge_cp S\<close> by auto
+      then show ?thesis using n_s \<open> cdcl\<^sub>W_merge_stgy\<^sup>*\<^sup>* R S\<close> unfolding full_def by auto
+    next
+      case fw_dec_no_confl
+      then have "full cdcl\<^sub>W_merge_cp T V"
+        using n_s_cp unfolding full_def by blast
+      then have "cdcl\<^sub>W_merge_stgy S V" using \<open>decide S T\<close> \<open>no_step cdcl\<^sub>W_merge_cp S\<close> by auto
+      then show ?thesis using n_s \<open> cdcl\<^sub>W_merge_stgy\<^sup>*\<^sup>* R S\<close> unfolding full_def by auto
+    next
+      case cp_no_confl
+      then have "full cdcl\<^sub>W_merge_cp R V"
+        by (simp add: full_def n_s_cp)
+      then have "R = V \<or> cdcl\<^sub>W_merge_stgy\<^sup>+\<^sup>+ R V"
+        using fw_s_cp unfolding full_unfold fw_s_cp
+        by (metis (no_types) rtranclp_unfold tranclp_unfold_end)
+      then show ?thesis
+        by (simp add: full_def n_s rtranclp_unfold)
+    next
+      case cp_confl
+      have "full cdcl\<^sub>W_bj V V"
+        using n_s_bj unfolding full_def by blast
+      then have "full1 cdcl\<^sub>W_merge_cp R V"
+        unfolding full1_def by (meson cdcl\<^sub>W_merge_cp.conflict' cp_confl(1,2) n_s_cp
+          rtranclp_into_tranclp1)
+      then show ?thesis using n_s unfolding full_def by auto
+    qed
+next
+  assume ?fw
+  then have "cdcl\<^sub>W\<^sup>*\<^sup>* R V" using rtranclp_mono[of cdcl\<^sub>W_merge_stgy "cdcl\<^sub>W\<^sup>*\<^sup>*"]
+    cdcl\<^sub>W_merge_stgy_rtranclp_cdcl\<^sub>W unfolding full_def by auto
+  then have inv': "cdcl\<^sub>W_all_struct_inv V" using inv rtranclp_cdcl\<^sub>W_all_struct_inv_inv by blast
+  have "cdcl\<^sub>W_s'\<^sup>*\<^sup>* R V"
+    using \<open>?fw\<close> by (simp add: full_def inv rtranclp_cdcl\<^sub>W_merge_stgy_rtranclp_cdcl\<^sub>W_s')
+  moreover have "no_step cdcl\<^sub>W_s' V"
+    proof cases
+      assume "conflicting V = None"
+      then show ?thesis
+        by (metis inv' \<open>full cdcl\<^sub>W_merge_stgy R V\<close> full_def
+          no_step_cdcl\<^sub>W_merge_stgy_no_step_cdcl\<^sub>W_s')
+    next
+      assume confl_V: "conflicting V \<noteq> None"
+      then have "no_step cdcl\<^sub>W_bj V"
+      using rtranclp_cdcl\<^sub>W_merge_stgy_no_step_cdcl\<^sub>W_bj by (meson \<open>full cdcl\<^sub>W_merge_stgy R V\<close>
+        assms(1) full_def)
+      then show ?thesis using confl_V by (fastforce simp: cdcl\<^sub>W_s'.simps full1_def cdcl\<^sub>W_cp.simps
+        dest!: tranclpD elim: rulesE)
+    qed
+  ultimately show ?s' unfolding full_def by blast
+qed
+
+lemma full_cdcl\<^sub>W_stgy_full_cdcl\<^sub>W_merge:
+  assumes
+    "conflicting R = None" and
+    inv: "cdcl\<^sub>W_all_struct_inv R"
+  shows "full cdcl\<^sub>W_stgy R V \<longleftrightarrow> full cdcl\<^sub>W_merge_stgy R V"
+  by (simp add: assms(1) full_cdcl\<^sub>W_s'_full_cdcl\<^sub>W_merge_restart full_cdcl\<^sub>W_stgy_iff_full_cdcl\<^sub>W_s'
+    inv)
 
 lemma full_cdcl\<^sub>W_merge_stgy_final_state_conclusive':
   fixes S' :: "'st"
@@ -545,562 +689,9 @@ proof -
   moreover have "conflicting (init_state N) = None"
     by auto
   ultimately show ?thesis
-    by (simp add: full full_cdcl\<^sub>W_stgy_final_state_conclusive_from_init_state
-      full_cdcl\<^sub>W_stgy_full_cdcl\<^sub>W_merge no_d)
+    using full full_cdcl\<^sub>W_stgy_final_state_conclusive_from_init_state
+    full_cdcl\<^sub>W_stgy_full_cdcl\<^sub>W_merge no_d by presburger
 qed
-
-end
-
-subsection \<open>Adding Restarts\<close>
-locale cdcl\<^sub>W_restart =
-  cdcl\<^sub>W trail init_clss learned_clss backtrack_lvl conflicting cons_trail tl_trail
-   add_init_cls
-   add_learned_cls remove_cls update_backtrack_lvl update_conflicting init_state
-   restart_state
-  for
-    trail :: "'st \<Rightarrow> ('v, nat, 'v clause) marked_lits" and
-    init_clss :: "'st \<Rightarrow> 'v clauses" and
-    learned_clss :: "'st \<Rightarrow> 'v clauses" and
-    backtrack_lvl :: "'st \<Rightarrow> nat" and
-    conflicting :: "'st \<Rightarrow>'v clause option" and
-
-    cons_trail :: "('v, nat, 'v clause) marked_lit \<Rightarrow> 'st \<Rightarrow> 'st" and
-    tl_trail :: "'st \<Rightarrow> 'st" and
-    add_init_cls :: "'v clause \<Rightarrow> 'st \<Rightarrow> 'st" and
-    add_learned_cls remove_cls :: "'v clause \<Rightarrow> 'st \<Rightarrow> 'st" and
-    update_backtrack_lvl :: "nat \<Rightarrow> 'st \<Rightarrow> 'st" and
-    update_conflicting :: "'v clause option \<Rightarrow> 'st \<Rightarrow> 'st" and
-
-    init_state :: "'v clauses \<Rightarrow> 'st" and
-    restart_state :: "'st \<Rightarrow> 'st" +
-  fixes f :: "nat \<Rightarrow> nat"
-  assumes f: "unbounded f"
-begin
-text \<open>The condition of the differences of cardinality has to be strict.
-  Otherwise, you could be in a strange state, where nothing remains to do, but a restart is done.
-  See the proof of well-foundedness.\<close>
-inductive cdcl\<^sub>W_merge_with_restart where
-restart_step:
-  "(cdcl\<^sub>W_merge_stgy^^(card (set_mset (learned_clss T)) - card (set_mset (learned_clss S)))) S T
-  \<Longrightarrow> card (set_mset (learned_clss T)) - card (set_mset (learned_clss S)) > f n
-  \<Longrightarrow> restart T U \<Longrightarrow> cdcl\<^sub>W_merge_with_restart (S, n) (U, Suc n)" |
-restart_full: "full1 cdcl\<^sub>W_merge_stgy S T \<Longrightarrow> cdcl\<^sub>W_merge_with_restart (S, n) (T, Suc n)"
-
-lemma "cdcl\<^sub>W_merge_with_restart S T \<Longrightarrow> cdcl\<^sub>W_merge_restart\<^sup>*\<^sup>* (fst S) (fst T)"
-  by (induction rule: cdcl\<^sub>W_merge_with_restart.induct)
-  (auto dest!: relpowp_imp_rtranclp cdcl\<^sub>W_merge_stgy_tranclp_cdcl\<^sub>W_merge tranclp_into_rtranclp
-     rtranclp_cdcl\<^sub>W_merge_stgy_rtranclp_cdcl\<^sub>W_merge rtranclp_cdcl\<^sub>W_merge_tranclp_cdcl\<^sub>W_merge_restart
-     fw_r_rf cdcl\<^sub>W_rf.restart
-    simp: full1_def)
-
-lemma cdcl\<^sub>W_merge_with_restart_rtranclp_cdcl\<^sub>W:
-  "cdcl\<^sub>W_merge_with_restart S T \<Longrightarrow> cdcl\<^sub>W\<^sup>*\<^sup>* (fst S) (fst T)"
-  by (induction rule: cdcl\<^sub>W_merge_with_restart.induct)
-  (auto dest!: relpowp_imp_rtranclp rtranclp_cdcl\<^sub>W_merge_stgy_rtranclp_cdcl\<^sub>W cdcl\<^sub>W.rf
-    cdcl\<^sub>W_rf.restart tranclp_into_rtranclp simp: full1_def)
-
-lemma cdcl\<^sub>W_merge_with_restart_increasing_number:
-  "cdcl\<^sub>W_merge_with_restart S T \<Longrightarrow> snd T = 1 + snd S"
-  by (induction rule: cdcl\<^sub>W_merge_with_restart.induct) auto
-
-lemma "full1 cdcl\<^sub>W_merge_stgy S T \<Longrightarrow> cdcl\<^sub>W_merge_with_restart (S, n) (T, Suc n)"
-  using restart_full by blast
-
-lemma cdcl\<^sub>W_all_struct_inv_learned_clss_bound:
-  assumes inv: "cdcl\<^sub>W_all_struct_inv S"
-  shows "set_mset (learned_clss S) \<subseteq> simple_clss (atms_of_mm (init_clss S))"
-proof
-  fix C
-  assume C: "C \<in> set_mset (learned_clss S)"
-  have "distinct_mset C"
-    using C inv unfolding cdcl\<^sub>W_all_struct_inv_def distinct_cdcl\<^sub>W_state_def distinct_mset_set_def
-    by auto
-  moreover have "\<not>tautology C"
-    using C inv unfolding cdcl\<^sub>W_all_struct_inv_def cdcl\<^sub>W_learned_clause_def by auto
-  moreover
-    have "atms_of C \<subseteq> atms_of_mm (learned_clss S)"
-      using C by auto
-    then have "atms_of C \<subseteq> atms_of_mm (init_clss S)"
-    using inv  unfolding cdcl\<^sub>W_all_struct_inv_def no_strange_atm_def by force
-  moreover have "finite (atms_of_mm (init_clss S))"
-    using inv unfolding cdcl\<^sub>W_all_struct_inv_def by auto
-  ultimately show "C \<in> simple_clss (atms_of_mm (init_clss S))"
-    using distinct_mset_not_tautology_implies_in_simple_clss simple_clss_mono
-    by blast
-qed
-
-lemma cdcl\<^sub>W_merge_with_restart_init_clss:
-  "cdcl\<^sub>W_merge_with_restart S T \<Longrightarrow> cdcl\<^sub>W_M_level_inv (fst S) \<Longrightarrow>
-  init_clss (fst S) = init_clss (fst T)"
-  using cdcl\<^sub>W_merge_with_restart_rtranclp_cdcl\<^sub>W rtranclp_cdcl\<^sub>W_init_clss by blast
-
-lemma
-  "wf {(T, S). cdcl\<^sub>W_all_struct_inv (fst S) \<and> cdcl\<^sub>W_merge_with_restart S T}"
-proof (rule ccontr)
-  assume "\<not> ?thesis"
-    then obtain g where
-    g: "\<And>i. cdcl\<^sub>W_merge_with_restart (g i) (g (Suc i))" and
-    inv: "\<And>i. cdcl\<^sub>W_all_struct_inv (fst (g i))"
-    unfolding wf_iff_no_infinite_down_chain by fast
-  { fix i
-    have "init_clss (fst (g i)) = init_clss (fst (g 0))"
-      apply (induction i)
-        apply simp
-      using g inv unfolding cdcl\<^sub>W_all_struct_inv_def by (metis cdcl\<^sub>W_merge_with_restart_init_clss)
-    } note init_g = this
-  let ?S = "g 0"
-  have "finite (atms_of_mm (init_clss (fst ?S)))"
-    using inv unfolding cdcl\<^sub>W_all_struct_inv_def by auto
-  have snd_g: "\<And>i. snd (g i) = i + snd (g 0)"
-    apply (induct_tac i)
-      apply simp
-    by (metis Suc_eq_plus1_left add_Suc cdcl\<^sub>W_merge_with_restart_increasing_number g)
-  then have snd_g_0: "\<And>i. i > 0 \<Longrightarrow> snd (g i) = i + snd (g 0)"
-    by blast
-  have unbounded_f_g: "unbounded (\<lambda>i. f (snd (g i)))"
-    using f unfolding bounded_def by (metis add.commute f less_or_eq_imp_le snd_g
-      not_bounded_nat_exists_larger not_le le_iff_add)
-
-  obtain k where
-    f_g_k: "f (snd (g k)) > card (simple_clss (atms_of_mm (init_clss (fst ?S))))" and
-    "k > card (simple_clss (atms_of_mm (init_clss (fst ?S))))"
-    using not_bounded_nat_exists_larger[OF unbounded_f_g] by blast
-  text \<open>The following does not hold anymore with the non-strict version of
-    cardinality in the definition.\<close>
-  { fix i
-    assume "no_step cdcl\<^sub>W_merge_stgy (fst (g i))"
-    with g[of i]
-    have False
-      proof (induction rule: cdcl\<^sub>W_merge_with_restart.induct)
-        case (restart_step T S n) note H = this(1) and c = this(2) and n_s = this(4)
-        obtain S' where "cdcl\<^sub>W_merge_stgy S S'"
-          using H c by (metis gr_implies_not0 relpowp_E2)
-        then show False using n_s by auto
-      next
-        case (restart_full S T)
-        then show False unfolding full1_def by (auto dest: tranclpD)
-      qed
-    } note H = this
-  obtain m T where
-    m: "m = card (set_mset (learned_clss T)) - card (set_mset (learned_clss (fst (g k))))" and
-    "m > f (snd (g k))" and
-    "restart T (fst (g (k+1)))" and
-    cdcl\<^sub>W_merge_stgy: "(cdcl\<^sub>W_merge_stgy ^^ m) (fst (g k)) T"
-    using g[of k] H[of "Suc k"] by (force simp: cdcl\<^sub>W_merge_with_restart.simps full1_def)
-  have "cdcl\<^sub>W_merge_stgy\<^sup>*\<^sup>* (fst (g k)) T"
-    using cdcl\<^sub>W_merge_stgy relpowp_imp_rtranclp by metis
-  then have "cdcl\<^sub>W_all_struct_inv T"
-    using inv[of k]  rtranclp_cdcl\<^sub>W_all_struct_inv_inv rtranclp_cdcl\<^sub>W_merge_stgy_rtranclp_cdcl\<^sub>W
-    by blast
-  moreover have "card (set_mset (learned_clss T)) - card (set_mset (learned_clss (fst (g k))))
-      > card (simple_clss (atms_of_mm (init_clss (fst ?S))))"
-      unfolding m[symmetric] using \<open>m > f (snd (g k))\<close> f_g_k by linarith
-    then have "card (set_mset (learned_clss T))
-      > card (simple_clss (atms_of_mm (init_clss (fst ?S))))"
-      by linarith
-  moreover
-    have "init_clss (fst (g k)) = init_clss T"
-      using \<open>cdcl\<^sub>W_merge_stgy\<^sup>*\<^sup>* (fst (g k)) T\<close> rtranclp_cdcl\<^sub>W_merge_stgy_rtranclp_cdcl\<^sub>W
-      rtranclp_cdcl\<^sub>W_init_clss inv unfolding cdcl\<^sub>W_all_struct_inv_def by blast
-    then have "init_clss (fst ?S) = init_clss T"
-      using init_g[of k] by auto
-  ultimately show False
-    using cdcl\<^sub>W_all_struct_inv_learned_clss_bound
-    by (simp add: \<open>finite (atms_of_mm (init_clss (fst (g 0))))\<close> simple_clss_finite
-      card_mono leD)
-qed
-
-lemma cdcl\<^sub>W_merge_with_restart_distinct_mset_clauses:
-  assumes invR: "cdcl\<^sub>W_all_struct_inv (fst R)" and
-  st: "cdcl\<^sub>W_merge_with_restart R S" and
-  dist: "distinct_mset (clauses (fst R))" and
-  R: "trail (fst R) = []"
-  shows "distinct_mset (clauses (fst S))"
-  using assms(2,1,3,4)
-proof (induction)
-  case (restart_full S T)
-  then show ?case using rtranclp_cdcl\<^sub>W_merge_stgy_distinct_mset_clauses[of S T] unfolding full1_def
-    by (auto dest: tranclp_into_rtranclp)
-next
-  case (restart_step T S n U)
-  then have "distinct_mset (clauses T)"
-    using rtranclp_cdcl\<^sub>W_merge_stgy_distinct_mset_clauses[of S T] unfolding full1_def
-    by (auto dest: relpowp_imp_rtranclp)
-  then show ?case using \<open>restart T U\<close> by (metis clauses_restart distinct_mset_union fstI
-    mset_le_exists_conv restart.cases state_eq_clauses)
-qed
-
-inductive cdcl\<^sub>W_with_restart where
-restart_step:
-  "(cdcl\<^sub>W_stgy^^(card (set_mset (learned_clss T)) - card (set_mset (learned_clss S)))) S T \<Longrightarrow>
-     card (set_mset (learned_clss T)) - card (set_mset (learned_clss S)) > f n \<Longrightarrow>
-     restart T U \<Longrightarrow>
-   cdcl\<^sub>W_with_restart (S, n) (U, Suc n)" |
-restart_full: "full1 cdcl\<^sub>W_stgy S T \<Longrightarrow> cdcl\<^sub>W_with_restart (S, n) (T, Suc n)"
-
-lemma cdcl\<^sub>W_with_restart_rtranclp_cdcl\<^sub>W:
-  "cdcl\<^sub>W_with_restart S T \<Longrightarrow> cdcl\<^sub>W\<^sup>*\<^sup>* (fst S) (fst T)"
-  apply (induction rule: cdcl\<^sub>W_with_restart.induct)
-  by (auto dest!: relpowp_imp_rtranclp  tranclp_into_rtranclp fw_r_rf
-     cdcl\<^sub>W_rf.restart rtranclp_cdcl\<^sub>W_stgy_rtranclp_cdcl\<^sub>W cdcl\<^sub>W_merge_restart_cdcl\<^sub>W
-    simp: full1_def)
-
-lemma cdcl\<^sub>W_with_restart_increasing_number:
-  "cdcl\<^sub>W_with_restart S T \<Longrightarrow> snd T = 1 + snd S"
-  by (induction rule: cdcl\<^sub>W_with_restart.induct) auto
-
-lemma "full1 cdcl\<^sub>W_stgy S T \<Longrightarrow> cdcl\<^sub>W_with_restart (S, n) (T, Suc n)"
-  using restart_full by blast
-
-lemma cdcl\<^sub>W_with_restart_init_clss:
-  "cdcl\<^sub>W_with_restart S T \<Longrightarrow>  cdcl\<^sub>W_M_level_inv (fst S) \<Longrightarrow> init_clss (fst S) = init_clss (fst T)"
-  using cdcl\<^sub>W_with_restart_rtranclp_cdcl\<^sub>W rtranclp_cdcl\<^sub>W_init_clss by blast
-
-lemma
-  "wf {(T, S). cdcl\<^sub>W_all_struct_inv (fst S) \<and> cdcl\<^sub>W_with_restart S T}"
-proof (rule ccontr)
-  assume "\<not> ?thesis"
-    then obtain g where
-    g: "\<And>i. cdcl\<^sub>W_with_restart (g i) (g (Suc i))" and
-    inv: "\<And>i. cdcl\<^sub>W_all_struct_inv (fst (g i))"
-    unfolding wf_iff_no_infinite_down_chain by fast
-  { fix i
-    have "init_clss (fst (g i)) = init_clss (fst (g 0))"
-      apply (induction i)
-        apply simp
-      using g inv unfolding cdcl\<^sub>W_all_struct_inv_def by (metis cdcl\<^sub>W_with_restart_init_clss)
-    } note init_g = this
-  let ?S = "g 0"
-  have "finite (atms_of_mm (init_clss (fst ?S)))"
-    using inv unfolding cdcl\<^sub>W_all_struct_inv_def by auto
-  have snd_g: "\<And>i. snd (g i) = i + snd (g 0)"
-    apply (induct_tac i)
-      apply simp
-    by (metis Suc_eq_plus1_left add_Suc cdcl\<^sub>W_with_restart_increasing_number g)
-  then have snd_g_0: "\<And>i. i > 0 \<Longrightarrow> snd (g i) = i + snd (g 0)"
-    by blast
-  have unbounded_f_g: "unbounded (\<lambda>i. f (snd (g i)))"
-    using f unfolding bounded_def by (metis add.commute f less_or_eq_imp_le snd_g
-      not_bounded_nat_exists_larger not_le le_iff_add)
-
-  obtain k where
-    f_g_k: "f (snd (g k)) > card (simple_clss (atms_of_mm (init_clss (fst ?S))))" and
-    "k > card (simple_clss (atms_of_mm (init_clss (fst ?S))))"
-    using not_bounded_nat_exists_larger[OF unbounded_f_g] by blast
-  text \<open>The following does not hold anymore with the non-strict version of
-    cardinality in the definition.\<close>
-  { fix i
-    assume "no_step cdcl\<^sub>W_stgy (fst (g i))"
-    with g[of i]
-    have False
-      proof (induction rule: cdcl\<^sub>W_with_restart.induct)
-        case (restart_step T S n) note H = this(1) and c = this(2) and n_s = this(4)
-        obtain S' where "cdcl\<^sub>W_stgy S S'"
-          using H c by (metis gr_implies_not0 relpowp_E2)
-        then show False using n_s by auto
-      next
-        case (restart_full S T)
-        then show False unfolding full1_def by (auto dest: tranclpD)
-      qed
-    } note H = this
-  obtain m T where
-    m: "m = card (set_mset (learned_clss T)) - card (set_mset (learned_clss (fst (g k))))" and
-    "m > f (snd (g k))" and
-    "restart T (fst (g (k+1)))" and
-    cdcl\<^sub>W_merge_stgy: "(cdcl\<^sub>W_stgy ^^ m) (fst (g k)) T"
-    using g[of k] H[of "Suc k"] by (force simp: cdcl\<^sub>W_with_restart.simps full1_def)
-  have "cdcl\<^sub>W_stgy\<^sup>*\<^sup>* (fst (g k)) T"
-    using cdcl\<^sub>W_merge_stgy relpowp_imp_rtranclp by metis
-  then have "cdcl\<^sub>W_all_struct_inv T"
-    using inv[of k]  rtranclp_cdcl\<^sub>W_all_struct_inv_inv rtranclp_cdcl\<^sub>W_stgy_rtranclp_cdcl\<^sub>W by blast
-  moreover have "card (set_mset (learned_clss T)) - card (set_mset (learned_clss (fst (g k))))
-      > card (simple_clss (atms_of_mm (init_clss (fst ?S))))"
-      unfolding m[symmetric] using \<open>m > f (snd (g k))\<close> f_g_k by linarith
-    then have "card (set_mset (learned_clss T))
-      > card (simple_clss (atms_of_mm (init_clss (fst ?S))))"
-      by linarith
-  moreover
-    have "init_clss (fst (g k)) = init_clss T"
-      using \<open>cdcl\<^sub>W_stgy\<^sup>*\<^sup>* (fst (g k)) T\<close> rtranclp_cdcl\<^sub>W_stgy_rtranclp_cdcl\<^sub>W rtranclp_cdcl\<^sub>W_init_clss
-      inv unfolding cdcl\<^sub>W_all_struct_inv_def
-      by blast
-    then have "init_clss (fst ?S) = init_clss T"
-      using init_g[of k] by auto
-  ultimately show False
-    using cdcl\<^sub>W_all_struct_inv_learned_clss_bound
-    by (simp add: \<open>finite (atms_of_mm (init_clss (fst (g 0))))\<close> simple_clss_finite
-      card_mono leD)
-qed
-
-lemma cdcl\<^sub>W_with_restart_distinct_mset_clauses:
-  assumes invR: "cdcl\<^sub>W_all_struct_inv (fst R)" and
-  st: "cdcl\<^sub>W_with_restart R S" and
-  dist: "distinct_mset (clauses (fst R))" and
-  R: "trail (fst R) = []"
-  shows "distinct_mset (clauses (fst S))"
-  using assms(2,1,3,4)
-proof (induction)
-  case (restart_full S T)
-  then show ?case using rtranclp_cdcl\<^sub>W_stgy_distinct_mset_clauses[of S T] unfolding full1_def
-    by (auto dest: tranclp_into_rtranclp)
-next
-  case (restart_step T S n U)
-  then have "distinct_mset (clauses T)" using rtranclp_cdcl\<^sub>W_stgy_distinct_mset_clauses[of S T]
-    unfolding full1_def by (auto dest: relpowp_imp_rtranclp)
-  then show ?case using \<open>restart T U\<close> by (metis clauses_restart distinct_mset_union fstI
-    mset_le_exists_conv restart.cases state_eq_clauses)
-qed
-end
-
-locale luby_sequence =
-  fixes ur :: nat (*unit run*)
-  assumes "ur > 0"
-begin
-
-lemma exists_luby_decomp:
-  fixes i ::nat
-  shows "\<exists>k::nat. (2 ^ (k - 1) \<le> i \<and> i < 2 ^ k - 1) \<or> i = 2 ^ k - 1"
-proof (induction i)
-  case 0
-  then show ?case
-    by (rule exI[of _ 0], simp)
-next
-  case (Suc n)
-  then obtain k where "2 ^ (k - 1) \<le> n \<and> n < 2 ^ k - 1 \<or> n = 2 ^ k - 1"
-    by blast
-  then consider
-      (st_interv) "2 ^ (k - 1) \<le> n" and  "n \<le> 2 ^ k - 2"
-    | (end_interv) "2 ^ (k - 1) \<le> n" and "n = 2 ^ k - 2"
-    | (pow2) "n = 2 ^ k - 1"
-    by linarith
-  then show ?case
-    proof cases
-      case st_interv
-      then show ?thesis apply - apply (rule exI[of _ k])
-        by (metis (no_types, lifting) One_nat_def Suc_diff_Suc Suc_lessI
-          \<open>2 ^ (k - 1) \<le> n \<and> n < 2 ^ k - 1 \<or> n = 2 ^ k - 1\<close> diff_self_eq_0
-          dual_order.trans le_SucI le_imp_less_Suc numeral_2_eq_2 one_le_numeral
-          one_le_power zero_less_numeral zero_less_power)
-    next
-      case end_interv
-      then show ?thesis apply - apply (rule exI[of _ k]) by auto
-    next
-      case pow2
-      then show ?thesis apply - apply (rule exI[of _ "k+1"]) by auto
-    qed
-qed
-
-text \<open>Luby sequences are defined by:
-   \<^item> @{term "(2::nat)^(k::nat)- 1"}, if @{term "i = 2^k - 1"}
-   \<^item> @{term "luby_sequence_core (i - (2::nat)^(k - 1) + 1)"}, if @{term "2^(k - 1) \<le> i"} and
-   @{term "i \<le> 2^k - 1"}
-
-Then the sequence is then scaled by a constant unit run (called @{term ur} here), strictly positive.
-\<close>
-function luby_sequence_core :: "nat \<Rightarrow> nat" where
-"luby_sequence_core i =
-  (if \<exists>k. i = 2^k - 1
-  then 2^((SOME k. i = 2^k - 1) - 1)
-  else luby_sequence_core (i - 2^((SOME k. 2^(k-1)\<le> i \<and> i < 2^k - 1) - 1) + 1))"
-by auto
-termination
-proof (relation "less_than", goal_cases)
-  case 1
-  then show ?case by auto
-next
-  case (2 i)
-  let ?k = "(SOME k. 2 ^ (k - 1) \<le> i \<and> i < 2 ^ k - 1)"
-  have "2 ^ (?k - 1) \<le> i \<and> i < 2 ^ ?k - 1"
-    apply (rule someI_ex)
-    using "2" exists_luby_decomp by blast
-  then show ?case
-    (* sledgehammer *)
-    proof -
-      have "\<forall>n na. \<not> (1::nat) \<le> n \<or> 1 \<le> n ^ na"
-        by (meson one_le_power)
-      then have f1: "(1::nat) \<le> 2 ^ (?k - 1)"
-        using one_le_numeral by blast
-      have f2: "i - 2 ^ (?k - 1) + 2 ^ (?k - 1) = i"
-        using \<open>2 ^ (?k - 1) \<le> i \<and> i < 2 ^ ?k - 1\<close> le_add_diff_inverse2 by blast
-      have f3: "2 ^ ?k - 1 \<noteq> Suc 0"
-        using f1 \<open>2 ^ (?k - 1) \<le> i \<and> i < 2 ^ ?k - 1\<close> by linarith
-      have "2 ^ ?k - (1::nat) \<noteq> 0"
-        using \<open>2 ^ (?k - 1) \<le> i \<and> i < 2 ^ ?k - 1\<close> gr_implies_not0 by blast
-      then have f4: "2 ^ ?k \<noteq> (1::nat)"
-        by linarith
-      have f5: "\<forall>n na. if na = 0 then (n::nat) ^ na = 1 else n ^ na = n * n ^ (na - 1)"
-        by (simp add: power_eq_if)
-      then have "?k \<noteq> 0"
-        using f4 by meson
-      then have "2 ^ (?k - 1) \<noteq> Suc 0"
-        using f5 f3 by presburger
-      then have "Suc 0 < 2 ^ (?k - 1)"
-        using f1 by linarith
-      then show ?thesis
-        using f2 less_than_iff by presburger
-    qed
-qed
-
-declare luby_sequence_core.simps[simp del]
-
-lemma two_pover_n_eq_two_power_n'_eq:
-  assumes H: "(2::nat) ^ (k::nat) - 1 = 2 ^ k' - 1"
-  shows "k' = k"
-proof -
-  have "(2::nat) ^ (k::nat) = 2 ^ k'"
-    using H by (metis One_nat_def Suc_pred zero_less_numeral zero_less_power)
-  then show ?thesis by simp
-qed
-
-lemma luby_sequence_core_two_power_minus_one:
-  "luby_sequence_core (2^k - 1) = 2^(k-1)" (is "?L = ?K")
-proof -
-  have decomp: "\<exists>ka. 2 ^ k - 1 = 2 ^ ka - 1"
-    by auto
-  have "?L = 2^((SOME k'. (2::nat)^k - 1 = 2^k' - 1) - 1)"
-    apply (subst luby_sequence_core.simps, subst decomp)
-    by simp
-  moreover have "(SOME k'. (2::nat)^k - 1 = 2^k' - 1) = k"
-    apply (rule some_equality)
-      apply simp
-      using two_pover_n_eq_two_power_n'_eq by blast
-  ultimately show ?thesis by presburger
-qed
-
-lemma different_luby_decomposition_false:
-  assumes
-    H: "2 ^ (k - Suc 0) \<le> i" and
-    k': "i < 2 ^ k' - Suc 0" and
-    k_k': "k > k'"
-  shows "False"
-proof -
-  have "2 ^ k' - Suc 0 < 2 ^ (k - Suc 0)"
-    using k_k' less_eq_Suc_le by auto
-  then show ?thesis
-    using H k' by linarith
-qed
-
-lemma luby_sequence_core_not_two_power_minus_one:
-  assumes
-    k_i: "2 ^ (k - 1) \<le> i" and
-    i_k: "i < 2^ k - 1"
-  shows "luby_sequence_core i = luby_sequence_core (i - 2 ^ (k - 1) + 1)"
-proof -
-  have H: "\<not> (\<exists>ka. i = 2 ^ ka - 1)"
-    proof (rule ccontr)
-      assume "\<not> ?thesis"
-      then obtain k'::nat where k': "i = 2 ^ k' - 1" by blast
-      have "(2::nat) ^ k' - 1 < 2 ^ k - 1"
-        using i_k unfolding k' .
-      then have "(2::nat) ^ k' < 2 ^ k"
-        by linarith
-      then have "k' < k"
-        by simp
-      have "2 ^ (k - 1) \<le> 2 ^ k' - (1::nat)"
-        using k_i unfolding k' .
-      then have "(2::nat) ^ (k-1) < 2 ^ k'"
-        by (metis Suc_diff_1 not_le not_less_eq zero_less_numeral zero_less_power)
-      then have "k-1 < k'"
-        by simp
-
-      show False using \<open>k' < k\<close> \<open>k-1 < k'\<close> by linarith
-    qed
-  have "\<And>k k'. 2 ^ (k - Suc 0) \<le> i \<Longrightarrow> i < 2 ^ k - Suc 0 \<Longrightarrow> 2 ^ (k' - Suc 0) \<le> i \<Longrightarrow>
-    i < 2 ^ k' - Suc 0 \<Longrightarrow> k = k'"
-    by (meson different_luby_decomposition_false linorder_neqE_nat)
-  then have k: "(SOME k. 2 ^ (k - Suc 0) \<le> i \<and> i < 2 ^ k - Suc 0) = k"
-    using k_i i_k by auto
-  show ?thesis
-    apply (subst luby_sequence_core.simps[of i], subst H)
-    by (simp add: k)
-qed
-
-lemma unbounded_luby_sequence_core: "unbounded luby_sequence_core"
-  unfolding bounded_def
-proof
-  assume "\<exists>b. \<forall>n. luby_sequence_core n \<le> b"
-  then obtain b where b: "\<And>n. luby_sequence_core n \<le> b"
-    by metis
-  have "luby_sequence_core (2^(b+1) - 1) = 2^b"
-    using luby_sequence_core_two_power_minus_one[of "b+1"] by simp
-  moreover have "(2::nat)^b > b"
-    by (induction b) auto
-  ultimately show False using b[of "2^(b+1) - 1"] by linarith
-qed
-
-abbreviation luby_sequence :: "nat \<Rightarrow> nat" where
-"luby_sequence n \<equiv>  ur * luby_sequence_core n"
-
-lemma bounded_luby_sequence: "unbounded luby_sequence"
-  using bounded_const_product[of ur] luby_sequence_axioms
-  luby_sequence_def unbounded_luby_sequence_core by blast
-
-lemma luby_sequence_core_0: "luby_sequence_core 0 = 1"
-proof -
-  have 0: "(0::nat) = 2^0-1"
-    by auto
-  show ?thesis
-    by (subst 0, subst luby_sequence_core_two_power_minus_one) simp
-qed
-
-lemma "luby_sequence_core n \<ge> 1"
-proof (induction n rule: nat_less_induct_case)
-  case 0
-  then show ?case by (simp add: luby_sequence_core_0)
-next
-  case (Suc n) note IH = this
-
-  consider
-      (interv) k where "2 ^ (k - 1) \<le> Suc n" and "Suc n < 2 ^ k - 1"
-    | (pow2)  k where "Suc n = 2 ^ k - Suc 0"
-    using exists_luby_decomp[of "Suc n"] by auto
-
-  then show ?case
-     proof cases
-       case pow2
-       show ?thesis
-         using luby_sequence_core_two_power_minus_one pow2 by auto
-     next
-       case interv
-       have n: "Suc n - 2 ^ (k - 1) + 1 < Suc n"
-         by (metis Suc_1 Suc_eq_plus1 add.commute add_diff_cancel_left' add_less_mono1 gr0I
-           interv(1) interv(2) le_add_diff_inverse2 less_Suc_eq not_le power_0 power_one_right
-           power_strict_increasing_iff)
-       show ?thesis
-         apply (subst luby_sequence_core_not_two_power_minus_one[OF interv])
-         using IH n by auto
-     qed
-qed
-end
-
-locale luby_sequence_restart =
-  luby_sequence ur +
-  cdcl\<^sub>W trail init_clss learned_clss backtrack_lvl conflicting cons_trail tl_trail
-    add_init_cls
-    add_learned_cls remove_cls update_backtrack_lvl update_conflicting init_state
-    restart_state
-  for
-    ur :: nat and
-    trail :: "'st \<Rightarrow> ('v, nat, 'v clause) marked_lits" and
-    init_clss :: "'st \<Rightarrow> 'v clauses" and
-    learned_clss :: "'st \<Rightarrow> 'v clauses" and
-    backtrack_lvl :: "'st \<Rightarrow> nat" and
-    conflicting :: "'st \<Rightarrow>'v clause option" and
-    cons_trail :: "('v, nat, 'v clause) marked_lit \<Rightarrow> 'st \<Rightarrow> 'st" and
-    tl_trail :: "'st \<Rightarrow> 'st" and
-    add_init_cls :: "'v clause \<Rightarrow> 'st \<Rightarrow> 'st" and
-    add_learned_cls remove_cls :: "'v clause \<Rightarrow> 'st \<Rightarrow> 'st" and
-    update_backtrack_lvl :: "nat \<Rightarrow> 'st \<Rightarrow> 'st" and
-    update_conflicting :: "'v clause option \<Rightarrow> 'st \<Rightarrow> 'st" and
-
-    init_state :: "'v clauses \<Rightarrow> 'st" and
-    restart_state :: "'st \<Rightarrow> 'st"
-begin
-
-sublocale cdcl\<^sub>W_restart _ _ _ _ _ _ _ _ _ _ _ _ _ _ luby_sequence
-  apply unfold_locales
-  using bounded_luby_sequence by blast
-
 end
 
 end
