Weidenbach_Book/Weidenbach_Book.thy
@@ -7,7 +7,7 @@ imports
   Prop_Superposition
 
   CDCL_NOT DPLL_NOT DPLL_W_Implementation CDCL_W_Implementation CDCL_W_Incremental
-  CDCL_WNOT CDCL_Two_Watched_Literals
+  CDCL_WNOT (* CDCL_Two_Watched_Literals *)
 
 begin
 
